AwsCryptographicMaterialProviders/dafny/AwsCryptographyKeyStoreAdmin/src/Mutations.dfy
@@ -4,9 +4,9 @@ include "../../AwsCryptographyKeyStore/src/KeyStoreErrorMessages.dfy"
 include "../Model/AwsCryptographyKeyStoreAdminTypes.dfy"
 include "MutationStateStructures.dfy"
 include "MutationErrorRefinement.dfy"
-include "KmsUtils.dfy"
+include "../../../dafny/AwsCryptographyKeyStore/src/KmsUtils.dfy"
+include "KeyStoreAdminHelpers.dfy"
 include "KeyStoreAdminErrorMessages.dfy"
-include "CreateKeysHV2.dfy"
 
 /** Common Functions/Methods for Mutations. */
 module {:options "/functionSyntax:4" } Mutations {
@@ -26,13 +26,13 @@ module {:options "/functionSyntax:4" } Mutations {
   import GetKeys
   import KeyStoreErrorMessages
   import HVUtils = HierarchicalVersionUtils
+  import KmsUtils
 
   import Types = AwsCryptographyKeyStoreAdminTypes
   import StateStrucs = MutationStateStructures
   import KeyStoreAdminErrorMessages
   import MutationErrorRefinement
-  import KmsUtils
-  import CreateKeysHV2
+  import KeyStoreAdminHelpers
 
   const StringToHierarchyVersion := Structure.StringToHierarchyVersion
   const HierarchyVersionToString := Structure.HierarchyVersionToString
@@ -106,6 +106,32 @@ module {:options "/functionSyntax:4" } Mutations {
   {
     var success?: bool := false;
     var throwAwayError;
+    if (mutationToApply.Terminal.hierarchyVersion.v2?) {
+      // TODO-HV-2-M2: Add test to cover the if condition of this code path
+      // TODO-HV-2-M4: Support other key manager strategy
+      :- Need(keyManagerStrategy.kmsSimple?, Types.UnsupportedFeatureException(message:=KeyStoreAdminErrorMessages.UNSUPPORTED_KEY_MANAGEMENT_STRATEGY_HV_2));
+      var decryptRes := GetKeys.DecryptBranchKeyItem(
+        item,
+        KeyStoreAdminHelpers.KmsSymmetricKeyArnToKMSConfiguration(Types.KmsSymmetricKeyArn.KmsKeyArn(item.KmsArn)),
+        keyManagerStrategy.kmsSimple.grantTokens,
+        keyManagerStrategy.kmsSimple.kmsClient
+      );
+      if decryptRes.Success? {
+        return Success(ActiveVerificationHolder.KmsDecrypt(decryptRes.value));
+      }
+      if decryptRes.error.ComAmazonawsKms? || decryptRes.error.KeyManagementException? || decryptRes.error.BranchKeyCiphertextException? {
+        var error := BuildVerificationError(
+          item,
+          decryptRes.error,
+          localOperation,
+          "Decrypt"
+        );
+        return Failure(error);
+      }
+      return Failure(Types.AwsCryptographyKeyStore(
+                       AwsCryptographyKeyStore := decryptRes.error
+                     ));
+    }
     var kmsOperation: string;
     match keyManagerStrategy {
       case reEncrypt(kms) =>
@@ -203,7 +229,7 @@ module {:options "/functionSyntax:4" } Mutations {
 
     var decryptRes := GetKeys.DecryptBranchKeyItem(
       item,
-      KmsUtils.KmsSymmetricKeyArnToKMSConfiguration(Types.KmsSymmetricKeyArn.KmsKeyArn(item.KmsArn)),
+      KeyStoreAdminHelpers.KmsSymmetricKeyArnToKMSConfiguration(Types.KmsSymmetricKeyArn.KmsKeyArn(item.KmsArn)),
       KMSTuple.grantTokens,
       KMSTuple.kmsClient
     );
@@ -675,7 +701,7 @@ module {:options "/functionSyntax:4" } Mutations {
       plainTextTuple,
       HVUtils.SelectKmsEncryptionContextForHv2(terminalBKC),
       terminalBKC[Structure.KMS_FIELD],
-      KmsUtils.KmsSymmetricKeyArnToKMSConfiguration(Types.KmsSymmetricKeyArn.KmsKeyArn(terminalBKC[Structure.KMS_FIELD])),
+      KeyStoreAdminHelpers.KmsSymmetricKeyArnToKMSConfiguration(Types.KmsSymmetricKeyArn.KmsKeyArn(terminalBKC[Structure.KMS_FIELD])),
       encryptKMSTuple.grantTokens,
       encryptKMSTuple.kmsClient
     );
@@ -714,7 +740,7 @@ module {:options "/functionSyntax:4" } Mutations {
               && var hv := item.EncryptionContext[Structure.HIERARCHY_VERSION];
               && GetKeys.ValidateKmsDecryption(
                    item,
-                   KmsUtils.KmsSymmetricKeyArnToKMSConfiguration(Types.KmsSymmetricKeyArn.KmsKeyArn(item.KmsArn)),
+                   KeyStoreAdminHelpers.KmsSymmetricKeyArnToKMSConfiguration(Types.KmsSymmetricKeyArn.KmsKeyArn(item.KmsArn)),
                    grantTokens,
                    kmsClient,
                    hv)
@@ -728,7 +754,7 @@ module {:options "/functionSyntax:4" } Mutations {
   {
     var decryptRes := GetKeys.DecryptBranchKeyItem(
       item,
-      KmsUtils.KmsSymmetricKeyArnToKMSConfiguration(Types.KmsSymmetricKeyArn.KmsKeyArn(item.KmsArn)),
+      KeyStoreAdminHelpers.KmsSymmetricKeyArnToKMSConfiguration(Types.KmsSymmetricKeyArn.KmsKeyArn(item.KmsArn)),
       grantTokens,
       kmsClient
     );
